Drop separate liftTT' and substTT' functions

proof/Poly/SubstTypeType.v
@@ -7,7 +7,7 @@ Require Import Base.
 
 (* Types ************************************************************)
 (* Lift type indices that are at least a certain depth. *)
-Fixpoint liftTT' (d: nat) (tt: ty) : ty :=
+Fixpoint liftTT (d: nat) (tt: ty) : ty :=
   match tt with
   | TCon _     => tt
 
@@ -17,14 +17,11 @@ Fixpoint liftTT' (d: nat) (tt: ty) : ty :=
       else tt
 
   |  TForall t 
-  => TForall (liftTT' (S d) t)
+  => TForall (liftTT (S d) t)
 
   |  TFun t1 t2
-  => TFun    (liftTT' d t1) (liftTT' d t2)
+  => TFun    (liftTT d t1) (liftTT d t2)
   end.
-Hint Unfold liftTT'.
-
-Definition liftTT  := liftTT' 0.
 Hint Unfold liftTT.
 
 Ltac liftTT_cases 
@@ -35,7 +32,7 @@ Ltac liftTT_cases
 
 
 (* Substitution of Types in Types. *)
-Fixpoint substTT' (d: nat) (u: ty) (tt: ty) : ty 
+Fixpoint substTT (d: nat) (u: ty) (tt: ty) : ty 
  := match tt with
     |  TCon _     
     => tt
@@ -48,29 +45,20 @@ Fixpoint substTT' (d: nat) (u: ty) (tt: ty) : ty
        end
 
     |  TForall t  
-    => TForall (substTT' (S d) (liftTT' 0 u) t)
+    => TForall (substTT (S d) (liftTT 0 u) t)
 
     |  TFun t1 t2 
-    => TFun (substTT' d u t1) (substTT' d u t2)
+    => TFun (substTT d u t1) (substTT d u t2)
   end.
-
-Definition substTT := substTT' 0.
-Hint Unfold substTT.
 
 
 (* Type Environments ************************************************)
 (* Lift type indices in type environments. *)
-Definition liftTE' d te    := map (liftTT' d) te.
-Hint Unfold liftTE'.
-
-Definition liftTE te       := liftTE' 0 te.
+Definition liftTE d te    := map (liftTT d) te.
 Hint Unfold liftTE.
 
 (* Substitution of Types in Type Environments. *)
-Definition substTE' d t te := map (substTT' d t) te.
-Hint Unfold substTE'.
-
-Definition substTE te      := substTE' 0 te.
+Definition substTE d t te := map (substTT d t) te.
 Hint Unfold substTE.
 
 
@@ -78,15 +66,15 @@ Hint Unfold substTE.
 (* Changing the order of lifting. *)
 Lemma liftTT_liftTT
  :  forall n n' t
- ,  liftTT' n              (liftTT' (n + n') t) 
- =  liftTT' (1 + (n + n')) (liftTT' n t).
+ ,  liftTT n              (liftTT (n + n') t) 
+ =  liftTT (1 + (n + n')) (liftTT n t).
 Proof.
  intros. gen n n'.
  induction t; intros; auto.
 
  Case "TVar".
   simpl.
-  repeat (unfold liftTT'; liftTT_cases; intros); burn.
+  repeat (unfold liftTT; liftTT_cases; intros); burn.
 
  Case "TForall".
   simpl.
@@ -102,13 +90,13 @@ Qed.
    substituting into it doens't do anything. *)
 Lemma substTT_liftTT
  :  forall d t1 t2
- ,  substTT' d t2 (liftTT' d t1) = t1.
+ ,  substTT d t2 (liftTT d t1) = t1.
 Proof.
  intros. gen d t2.
  induction t1; intros; eauto.
 
  Case "TVar".
-  simpl; liftTT_cases; unfold substTT';
+  simpl; liftTT_cases; unfold substTT;
    fbreak_nat_compare; intros;
    burn.
 
@@ -126,8 +114,8 @@ Qed.
 (* Lifting after substitution *)
 Lemma liftTT_substTT
  :  forall n n' t1 t2
- ,  liftTT' n (substTT' (n + n') t2 t1)
- =  substTT' (1 + n + n') (liftTT' n t2) (liftTT' n t1).
+ ,  liftTT n (substTT (n + n') t2 t1)
+ =  substTT (1 + n + n') (liftTT n t2) (liftTT n t1).
 Proof.
  intros. gen n n' t2.
  induction t1; intros; eauto.
@@ -152,9 +140,9 @@ Qed.
 (* Commuting substitutions. *)
 Lemma substTT_substTT
  :  forall n m t1 t2 t3
- ,  substTT' (n + m) t3 (substTT' n t2 t1)
- =  substTT' n (substTT' (n + m) t3 t2)
-               (substTT' (1 + n + m) (liftTT' n t3) t1).
+ ,  substTT (n + m) t3 (substTT n t2 t1)
+ =  substTT n (substTT (n + m) t3 t2)
+              (substTT (1 + n + m) (liftTT n t3) t1).
 Proof.
  intros. gen n m t2 t3.
  induction t1; intros; auto.
@@ -179,15 +167,15 @@ Qed.
 (* Lifting lemmas on environments ***********************************)
 Lemma liftTE_substTE
  :  forall n n' t2 te
- ,  liftTE' n (substTE' (n + n') t2 te)
- =  substTE' (1 + n + n') (liftTT' n t2) (liftTE' n te).
+ ,  liftTE n (substTE (n + n') t2 te)
+ =  substTE (1 + n + n') (liftTT n t2) (liftTE n te).
 Proof.
  intros. induction te.
   auto.
-  unfold substTE'. unfold liftTE'.
+  unfold substTE. unfold liftTE.
    simpl. rewrite liftTT_substTT.
-   unfold liftTE' in IHte.
-   unfold substTE' in IHte. rewrite IHte. auto.
+   unfold liftTE in IHte.
+   unfold substTE in IHte. rewrite IHte. auto.
 Qed.
 
 
@@ -195,7 +183,7 @@ Qed.
 Lemma liftTT_insert
  :  forall ke ix t k1 k2
  ,  KIND ke t k1
- -> KIND (insert ix k2 ke) (liftTT' ix t) k1.
+ -> KIND (insert ix k2 ke) (liftTT ix t) k1.
 Proof.
  intros. gen ix ke k1.
  induction t; intros; simpl; inverts H; eauto.
@@ -212,8 +200,8 @@ Qed.
 
 Lemma liftTT_push
  :  forall ke t k1 k2
- ,  KIND  ke         t         k1
- -> KIND (ke :> k2) (liftTT t) k1.
+ ,  KIND  ke         t           k1
+ -> KIND (ke :> k2) (liftTT 0 t) k1.
 Proof.
  intros.
  assert (ke :> k2 = insert 0 k2 ke). simpl.
@@ -233,7 +221,7 @@ Theorem subst_type_type_ix
  ,  get ke ix = Some k2
  -> KIND ke t1 k1
  -> KIND (drop ix ke) t2 k2
- -> KIND (drop ix ke) (substTT' ix t2 t1) k1.
+ -> KIND (drop ix ke) (substTT ix t2 t1) k1.
 Proof.
  intros. gen ix ke t2 k1 k2.
  induction t1; intros; simpl; inverts H0; eauto.
@@ -266,7 +254,7 @@ Theorem subst_type_type
  :  forall ke t1 k1 t2 k2
  ,  KIND (ke :> k2) t1 k1
  -> KIND ke         t2 k2
- -> KIND ke (substTT t2 t1) k1.
+ -> KIND ke (substTT 0 t2 t1) k1.
 Proof.
  intros.
  unfold substTT.
