proof/Poly/SubstTypeValue.v
@@ -8,45 +8,41 @@ Require Import Base.
 
 
 (* Lift type indices that are at least a certain depth. *)
-Fixpoint liftTX' (d: nat) (xx: exp) : exp :=
+Fixpoint liftTX (d: nat) (xx: exp) : exp :=
   match xx with
   |  XVar _     => xx
 
   |  XLAM x     
-  => XLAM (liftTX' (S d) x)
+  => XLAM (liftTX (S d) x)
 
   |  XAPP x t 
-  => XAPP (liftTX' d x)  (liftTT' d t)
+  => XAPP (liftTX d x)  (liftTT d t)
  
   |  XLam t x   
-  => XLam (liftTT' d t)  (liftTX' d x)
+  => XLam (liftTT d t)  (liftTX d x)
 
   |  XApp x1 x2
-  => XApp (liftTX' d x1) (liftTX' d x2)
+  => XApp (liftTX d x1) (liftTX d x2)
  end.
 
 
 (* Substitution of Types in Exps *)
-Fixpoint substTX' (d: nat) (u: ty) (xx: exp) : exp :=
+Fixpoint substTX (d: nat) (u: ty) (xx: exp) : exp :=
   match xx with
   | XVar _     => xx
 
   |  XLAM x     
-  => XLAM (substTX' (S d) (liftTT' 0 u) x)
+  => XLAM (substTX (S d) (liftTT 0 u) x)
 
   |  XAPP x t
-  => XAPP (substTX' d u x)  (substTT' d u t)
+  => XAPP (substTX d u x)  (substTT d u t)
 
   |  XLam t x
-  => XLam (substTT' d u t)  (substTX' d u x)
+  => XLam (substTT d u t)  (substTX d u x)
 
   |  XApp x1 x2
-  => XApp (substTX' d u x1) (substTX' d u x2)
+  => XApp (substTX d u x1) (substTX d u x2)
  end.
-
-
-Definition  substTX := substTX' 0.
-Hint Unfold substTX.
 
 
 Theorem subst_type_value_ix
@@ -55,16 +51,16 @@ Theorem subst_type_value_ix
  -> TYPE ke  te x1 t1
  -> KIND (drop ix ke)  t2 k2
  -> TYPE (drop ix ke) 
-         (substTE' ix t2 te)
-         (substTX' ix t2 x1)
-         (substTT' ix t2 t1).
+         (substTE ix t2 te)
+         (substTX ix t2 x1)
+         (substTT ix t2 t1).
 Proof.
  intros. gen ix ke te t1 t2 k2.
  induction x1; intros; simpl; inverts H0; eauto.
 
  Case "XVar".
   apply TYVar.
-  unfold substTE'. auto.
+  unfold substTE. auto.
 
  Case "XLAM".
   simpl. apply TYLAM.
@@ -81,9 +77,9 @@ Proof.
   
  Case "XLam".
   simpl. apply TYLam.
-  unfold substTE'. rewrite map_rewind.
-  assert ( map (substTT' ix t2) (te :> t)
-         = substTE' ix t2 (te :> t)). auto.
+  unfold substTE. rewrite map_rewind.
+  assert ( map (substTT ix t2) (te :> t)
+         = substTE ix t2 (te :> t)). auto.
   rewrite H0.
    eapply IHx1; eauto.
 
@@ -98,9 +94,9 @@ Theorem subst_type_value
  :  forall ke te x1 t1 t2 k2
  ,  TYPE (ke :> k2) te x1 t1
  -> KIND ke  t2 k2
- -> TYPE ke (substTE t2 te)
-            (substTX t2 x1)
-            (substTT t2 t1).
+ -> TYPE ke (substTE 0 t2 te)
+            (substTX 0 t2 x1)
+            (substTT 0 t2 t1).
 Proof.
  intros. 
  assert (ke = drop 0 (ke :> k2)). auto. rewrite H1.
